wip generalize
Modified-by: Aleksey Uymanov <s9gf4ult@gmail.com>

Projects.v
@@ -7,27 +7,44 @@ Inductive Project : Set :=
 | Seq : Project -> Project -> Project
 .
 
-Inductive Exec : Project -> nat -> nat -> Prop :=
-| ETask : forall (tid ord : nat), Exec (Task tid) ord ord
+Class is_time time :=
+  mk_is_time
+    { tle : time -> time -> Prop ; (* Time is less or equal than *)
+      tle_refl : forall a, tle a a ;
+      tle_transitive : forall a b c, tle a b -> tle b c -> tle a c ;
+      tmin : time -> time -> time ; (* Time min *)
+      tmin_commut : forall a b, tmin a b = tmin b a ;
+      tmax : time -> time -> time ; (* Time max *)
+      tmax_commut : forall a b, tmax a b = tmax b a ;
+      tle_min_max : forall a b c d, tle a c -> tle b d -> tle (tmin a b) (tmax c d) ;
+    }.
+
+Inductive Exec {time : Type} {isTime : is_time time} : Project -> time -> time -> Prop :=
+| ETask : forall tid t, Exec (Task tid) t t
 | ESumLeft : forall a b lo hi, Exec a lo hi -> Exec (Sum a b) lo hi
 | ESumRight : forall a b lo hi, Exec b lo hi -> Exec (Sum a b) lo hi
 | EProd : forall a b loA loB hiA hiB,
     Exec a loA hiA ->
     Exec b loB hiB ->
-    Exec (Prod a b) (min loA loB) (max hiA hiB)
+    Exec (Prod a b) (tmin loA loB) (tmax hiA hiB)
 | ESeq : forall a b loA loB hiA hiB,
     Exec a loA hiA ->
     Exec b loB hiB ->
-    hiA < loB      ->
+    tle hiA loB      ->
     Exec (Seq a b) loA hiB
 .
 
+
+
 (* a is less than b. If b is executed, then a is also executed *)
-Definition projLe a b : Type := (exists lo1 hi1, Exec b lo1 hi1) -> (exists lo2 hi2, Exec a lo2 hi2).
+Definition projLe {time} {isTime : is_time time} a b :=
+  (exists lo1 hi1, @Exec time isTime b lo1 hi1) ->
+  (exists lo2 hi2, @Exec time isTime a lo2 hi2).
 
-Definition projGe a b : Type := projLe b a.
+Definition projGe {time} {isTime : is_time time} a b := projLe b a.
 
-Definition projE a b : Type := projLe a b * projGe a b.
+Definition projE {time} {isTime : is_time time} a b :=
+  (projLe a b) /\ (projGe a b).
 
 Bind Scope proj_scope with Project.
 Delimit Scope proj_scope with proj.
@@ -44,62 +61,6 @@ Notation "a '<=' b" := (projLe a b) (at level 70) : proj_scope.
 Notation "a '>=' b" := (projGe b a) (at level 70) : proj_scope.
 
 Notation "a '<=>' b" := (projE a b) (at level 70) : proj_scope.
-
-Open Scope nat.
-Lemma minLeMax : forall (a b c d : nat) ,
-    a <= c ->
-    b <= d ->
-    min a b <= max c d.
-Proof.
-  intros.
-  destruct (a <=? b) eqn:AB. {
-    apply leb_complete in AB.
-    assert (ABmin: min a b = a) by (apply min_l ; assumption).
-    rewrite ABmin.
-    destruct (c <=? d) eqn:CD. {
-      apply leb_complete in CD.
-      assert (CDmax : max c d = d) by (apply max_r ; assumption).
-      rewrite CDmax.
-      omega.
-    } {
-      rewrite leb_iff_conv in CD.
-      assert (CDmax: max c d = c) by (apply max_l ; omega).
-      rewrite CDmax.
-      omega.
-    }
-  } {
-    apply leb_iff_conv in AB.
-    assert (ABmin: min a b = b) by (apply min_r ; omega).
-    rewrite ABmin.
-    destruct (c <=? d) eqn:CD. {
-      apply leb_complete in CD.
-      assert (CDmax : max c d = d) by (apply max_r ; assumption).
-      rewrite CDmax.
-      omega.
-    } {
-      rewrite leb_iff_conv in CD.
-      assert (CDmax: max c d = c) by (apply max_l ; omega).
-      rewrite CDmax.
-      omega.
-    }
-  }
-Qed.
-Close Scope nat.
-
-Lemma execHiLo : forall a lo hi, Exec a lo hi -> (lo <= hi)%nat.
-Proof.
-  intros.
-  induction H ; subst ; try omega.
-  - apply minLeMax ; assumption. (* EProd *)
-Qed.
-
-Lemma projESymmetry : forall a b, a <=> b -> b <=> a.
-Proof.
-  unfold projE, projGe, projLe.
-  intros.
-  inversion H.
-  constructor ; assumption.
-Qed.
 
 Ltac unfoldproj := unfold projE, projGe, projLe.
 
@@ -121,6 +82,211 @@ Ltac findExec :=
   | H : Exec ?a _ _ |- Exec (_ :+ (?a :+ _)) _ _ => apply ESumRight ; apply ESumLeft; apply H
   | H : Exec ?a _ _ |- Exec (_ :+ (_ :+ ?a)) _ _ => apply ESumRight ; apply ESumRight; apply H
   end.
+
+Ltac applyExEx :=
+  lazymatch goal with
+  |   Ex: Exec ?a _ _
+          , f : ((exists lo1 hi1, Exec ?a lo1 hi1)
+                 -> exists lo2 hi2, Exec ?b lo2 hi2)
+      |- _
+      => assert (exists lo hi, Exec b lo hi)
+         ; [ apply f ; eexistsall ; apply Ex | clear f]
+  end.
+
+
+
+Section Lemmas.
+  Context {time : Type}.
+  Context {isTime : is_time time}.
+
+  Lemma tle_min : forall a b c, tle a b -> tle (tmin a c) (tmax b c).
+  Proof.
+    intros.
+    apply tle_min_max ; try assumption.
+    - apply tle_refl.
+  Qed.
+
+  Lemma min_max : forall a b, tle (tmin a b) (tmax a b).
+  Proof.
+    intros.
+    apply tle_min_max ; apply tle_refl.
+  Qed.
+
+  Lemma execHiLo : forall a lo hi, Exec a lo hi -> tle lo hi.
+  Proof.
+    intros.
+    induction H ; try assumption. {
+      apply tle_refl.
+    } {
+      apply tle_min_max ; assumption.
+    } {
+      eapply tle_transitive. {
+        eapply tle_transitive.
+        - apply IHExec1.
+        - apply H1.
+      }
+      - assumption.
+    }
+  Qed.
+
+  Lemma projESymmetry : forall a b, a <=> b -> b <=> a.
+  Proof.
+    unfold projE, projGe, projLe.
+    intros.
+    inversion H.
+    constructor ; assumption.
+  Qed.
+
+  Lemma leTransitive : forall (a b c : Project), a <= b -> b <= c -> a <= c.
+  Proof.
+    unfoldproj.
+    intros.
+    auto.
+  Qed.
+
+  Lemma sumSymmetry : forall a b, a :+ b <=> b :+ a.
+  Proof.
+    unfoldproj.
+    intros.
+    split ; intros ; destructexists ; eexistsall
+    ; inversion H ; subst ; findExec.
+  Qed.
+
+  Lemma sumTransitive : forall a b c, a :+ (b :+ c) <= (a :+ b) :+ c .
+  Proof.
+    unfoldproj.
+    intros.
+    destructexists.
+    eexistsall.
+    inversion H ; subst. {
+      inversion H4 ; subst ; findExec.
+    } {
+      findExec.
+    }
+  Qed.
+
+  Lemma prodSymmetry : forall a b, a :* b <=> b :* a.
+  Proof.
+    unfoldproj.
+    intros.
+    split ; intros ; destructexists ;
+      inversion H ; subst ;
+      remember (tmin loB loA) as lo eqn:Le ;
+      remember (tmax hiB hiA) as hi eqn:He ;
+      exists lo, hi ;
+      rewrite Le;  rewrite He;
+      eapply EProd ; assumption.
+  Qed.
+
+  Lemma prodTransitive : forall a b c, a :* (b :* c) <=> (a :* b) :* c .
+  Proof.
+    unfoldproj.
+    intros.
+    split ; intros ; destructexists ; inversion H ; subst. {
+      inversion H2. subst.
+      eexistsall.
+      constructor ; try findExec ; try constructor ; findExec.
+    } {
+      inversion H5. subst.
+      eexistsall.
+      constructor ; try findExec ; try constructor ; findExec.
+    }
+  Qed.
+
+  Lemma sumDistrib : forall a b c, a :* (b :+ c) <=> a :* b :+ a :* c.
+  Proof.
+    unfoldproj.
+    intros.
+    split; intros ; destructexists. {
+      inversion H. {
+        inversion H4. subst.
+        eexistsall.
+        constructor ; try findExec; try findExec.
+      } {
+        inversion H4. subst.
+        eexistsall.
+        constructor ; try findExec; try findExec.
+      }
+    } {
+      inversion H ; subst.
+      inversion H5 ; subst; eexistsall. {
+        apply ESumLeft. constructor ; findExec.
+      } {
+        apply ESumRight. constructor ; findExec.
+      }
+    }
+  Qed.
+
+  Lemma seqTransitive : forall a b c, a :> (b :> c) <=> (a :> b) :> c.
+  Proof.
+    unfoldproj.
+    intros.
+    split ; intros; destructexists. {
+      inversion H ; subst.
+      inversion H2 ; subst.
+      eexistsall.
+      eapply ESeq.
+      - findExec.
+      - eapply ESeq ; try findExec ; assumption.
+      - assumption.
+    } {
+      inversion H ; subst.
+      inversion H3 ; subst.
+      eexistsall.
+      eapply ESeq.
+      - eapply ESeq; try findExec ; assumption.
+      - findExec.
+      - assumption.
+    }
+  Qed.
+
+  Lemma prodReduce : forall a b c d ,
+      (a <= c) + (a <= d) ->
+      (b <= c) + (b <= d) ->
+      a :* b <= c :* d.
+  Proof.
+    unfoldproj.
+    intros.
+    destruct H ; destruct H0 ;
+      destructexists ;
+      inversion H ; subst ;
+        applyExEx ;
+        applyExEx ;
+        destructexists ;
+        eexistsall ;
+        constructor ; findExec.
+  Qed.
+
+  Lemma sumReduce : forall a b c d,
+      (a <= c) + (b <= c) ->
+      (a <= d) + (b <= d) ->
+      a :+ b <= c :+ d.
+  Proof.
+    unfoldproj.
+    intros.
+    destruct H ; destruct H0 ; destructexists ;
+      inversion H ; subst;
+        applyExEx;
+        destructexists;
+        eexistsall; findExec.
+  Qed.
+End Lemmas.
+
+
+Instance natIsTime : is_time nat.
+Proof.
+  eapply mk_is_time. {
+    apply le_n.
+  } {
+    apply Nat.le_trans.
+  } {
+    apply Nat.min_comm.
+  } {
+    apply Nat.max_comm.
+  } {
+
+  }
+
 
 Fixpoint execute' (acc : nat) (p : Project) : exists lo hi, (Exec p lo hi /\ (lo > acc)%nat).
 Proof.
@@ -146,7 +312,7 @@ Proof.
     split. {
       constructor ; findExec.
     } {
-      unfold gt in *.
+      unfold gt, lt in *.
       apply Nat.min_glb_lt ; assumption.
     }
   } {
@@ -172,156 +338,4 @@ Proof.
   destruct H.
   eexistsall.
   findExec.
-Qed.
-
-(* This is fail, it must not be provable *)
-Lemma failure : forall a b, a <= b.
-Proof.
-  intros.
-  unfoldproj.
-  intros.
-  apply execute.
-Qed.
-
-Lemma leTransitive : forall (a b c : Project), a <= b -> b <= c -> a <= c.
-Proof.
-  unfoldproj.
-  intros.
-  auto.
-Qed.
-
-Lemma sumSymmetry : forall a b, a :+ b <=> b :+ a.
-Proof.
-  unfoldproj.
-  intros.
-  split ; intros ; destructexists ; eexistsall
-    ; inversion H ; subst ; findExec.
-Qed.
-
-Lemma sumTransitive : forall a b c, a :+ (b :+ c) <= (a :+ b) :+ c .
-Proof.
-  unfoldproj.
-  intros.
-  destructexists.
-  eexistsall.
-  inversion H ; subst. {
-    inversion H4 ; subst ; findExec.
-  } {
-    findExec.
-  }
-Qed.
-
-Lemma prodSymmetry : forall a b, a :* b <=> b :* a.
-Proof.
-  unfoldproj.
-  intros.
-  split ; intros ; destructexists ;
-    inversion H ; subst ;
-    remember (Init.Nat.min loB loA) as lo eqn:Le ;
-    remember (Init.Nat.max hiB hiA) as hi eqn:He ;
-    exists lo, hi ;
-    rewrite Le;  rewrite He;
-     eapply EProd ; assumption.
-Qed.
-
-Lemma prodTransitive : forall a b c, a :* (b :* c) <=> (a :* b) :* c .
-Proof.
-  unfoldproj.
-  intros.
-  split ; intros ; destructexists ; inversion H ; subst. {
-    inversion H2. subst.
-    eexistsall.
-    constructor ; try findExec ; try constructor ; findExec.
-  } {
-    inversion H5. subst.
-    eexistsall.
-    constructor ; try findExec ; try constructor ; findExec.
-  }
-Qed.
-
-Lemma sumDistrib : forall a b c, a :* (b :+ c) <=> a :* b :+ a :* c.
-Proof.
-  unfoldproj.
-  intros.
-  split; intros ; destructexists. {
-    inversion H. {
-      inversion H4. subst.
-      eexistsall.
-      constructor ; try findExec; try findExec.
-    } {
-      inversion H4. subst.
-      eexistsall.
-      constructor ; try findExec; try findExec.
-    }
-  } {
-    inversion H ; subst.
-    inversion H5 ; subst; eexistsall. {
-      apply ESumLeft. constructor ; findExec.
-    } {
-      apply ESumRight. constructor ; findExec.
-    }
-  }
-Qed.
-
-Lemma seqTransitive : forall a b c, a :> (b :> c) <=> (a :> b) :> c.
-Proof.
-  unfoldproj.
-  intros.
-  split ; intros; destructexists. {
-    inversion H ; subst.
-    inversion H2 ; subst.
-    eexistsall.
-    eapply ESeq.
-    - findExec.
-    - eapply ESeq ; try findExec ; assumption.
-    - assumption.
-  } {
-    inversion H ; subst.
-    inversion H3 ; subst.
-    eexistsall.
-    eapply ESeq.
-    - eapply ESeq; try findExec ; assumption.
-    - findExec.
-    - assumption.
-  }
-Qed.
-
-Ltac applyExEx :=
-  lazymatch goal with
-  |   Ex: Exec ?a _ _
-    , f : ((exists lo1 hi1 : nat, Exec ?a lo1 hi1)
-           -> exists lo2 hi2 : nat, Exec ?b lo2 hi2)
-    |- _
-    => assert (exists lo hi : nat, Exec b lo hi) ; [ apply f ; eexistsall ; apply Ex | clear f]
-  end.
-
-Lemma prodReduce : forall a b c d ,
-    (a <= c) + (a <= d) ->
-    (b <= c) + (b <= d) ->
-    a :* b <= c :* d.
-Proof.
-  unfoldproj.
-  intros.
-  destruct H ; destruct H0 ;
-    destructexists ;
-    inversion H ; subst ;
-    applyExEx ;
-    applyExEx ;
-    destructexists ;
-    eexistsall ;
-    constructor ; findExec.
-Qed.
-
-Lemma sumReduce : forall a b c d,
-    (a <= c) + (b <= c) ->
-    (a <= d) + (b <= d) ->
-    a :+ b <= c :+ d.
-Proof.
-  unfoldproj.
-  intros.
-  destruct H ; destruct H0 ; destructexists ;
-    inversion H ; subst;
-    applyExEx;
-    destructexists;
-    eexistsall; findExec.
 Qed.
